Resolve.v
@@ -16,11 +16,10 @@ Section Resolve.
 Variable maxReg : nat.          (* max number of registers *)
 Definition PhysReg : predArgType := 'I_maxReg.
 
-Variables blockType1 blockType2 opType1 opType2 varType accType : Set.
+Variables blockType1 blockType2 opType1 opType2 accType : Set.
 
 Variable binfo : BlockInfo blockType1 blockType2 opType1 opType2.
-Variable oinfo : OpInfo maxReg accType opType1 opType2 varType.
-Variable vinfo : VarInfo varType.
+Variable oinfo : OpInfo maxReg accType opType1 opType2.
 
 Definition checkIntervalBoundary `(st : @ScanState maxReg InUse sd)
   key in_from from to mappings vid :=
